\usepackage{amsmath}
\usepackage{amssymb}
\usepackage{autofe}
\usepackage{bbm}
\usepackage[greek,english]{babel}
\usepackage{etex}
\usepackage{framed}
\usepackage[utf8x]{inputenc}
\usepackage{proof}
\usepackage{stmaryrd}
\usepackage{suffix}
\usepackage{textalpha}
\usepackage{todo}
\usepackage{ucs}

\input{unicode}

\newcommand{\AgdaHide}[1]{}

\begin{document}

\maketitle

\section{Introduction}

According to the traditional approach to type theory \todo{Citation}, a type theory should have the
following properties in order to enjoy a good meaning explanation:
\begin{itemize}
\item \textbf{Confluence} --- The reduction relation should be confluent.
\item \textbf{Normalization} --- Every well-typed term should reduce to a normal form.
\item \textbf{Canonicity} --- Hence every well-typed term of type $A$ reduces to a unique canonical form of $A$.  (For example,
every closed term of type $\mathbb{N}$ reduces to a unique \emph{numeral} --- a term formed by applying $\mathrm{suc}$ some
finite number of times to 0.)
\end{itemize}

It is desirable to have, in addition, \emph{strong normalization}, so that we know that we are free to choose whatever reduction strategy we please.

The \emph{univalence axiom} of Homotopy Type theory (HoTT) \todo{Citation} breaks the property of canonicity.  It postulates a
constant
\[ \isotoid : A \simeq B \rightarrow A = B \]
that is an inverse to the canonical function $A = B \rightarrow A \simeq B$.  When a computation reaches a point
where we eliminate a path (proof of equality) formed by $\isotoid$, it gets 'stuck'.

As possible solutions to this problem, we may try to do with a weaker property than canonicity, such as \emph{propositional canonicity}.
We may attempt to prove that every closed term of type $\mathbb{N}$ is \emph{propositionally} equal to a numeral.  (This is known as
\emph{Voevodsky's Conecture} \todo{Cite}.)  Or we may attempt to change the definition of equality to make $\isotoid$ definable (\cite{Polonsky14a}), or
shift to an entirely different type theory such as Cubical Type Theory \todo{Cite}.

We could also try a more conservative approach, and simply attempt to find a reduction relation for a type theory involving $\isotoid$ that satisfies
all three of the properties above.  There seems to be no reason \emph{a priori} to believe this is not possible, but it is difficult to do because
the full Homotopy Type Theory is a complex and interdependent system.  We can tackle the problem by adding univalence to a much simpler system, finding
a well-behaved reduction relation, then doing the same for more and more complex systems, gradually approaching the full strength of HoTT.

In this paper, we present a system we call $\lambda o e$, or predicative higher-order propositional logic.  It is a type theory with two universes: the universe $\Omega$
of \emph{propositions}, and the universe of \emph{types}.  The propositions are closed under $\supset$ (implication) and include $\bot$ (falsehood), and an equality proposition $M =_A N$ for
any type $A$ and terms $M : A$ and $N : A$.  The types include $\Omega$ itself and are closed under $\rightarrow$ (non-dependent function type).

There are two canonical forms for proofs of $M =_\Omega N$.  For any term $M : \Omega$, we have $\reff{M} : M =_\Omega M$.  We also add univalence for this system, in this form:
if $\delta : \phi \supset \psi$ and $\epsilon : \psi \supset\phi$, then $\univ{\phi}{\psi}{\delta}{\epsilon} : \phi =_\Omega \psi$.  

We present a reduction relation for this system, and prove it satisfies confluence, strong normalization and canonicity. \todo{Cross-reference lemma numbers.}

For the future, we wish to expand the system with universal quantification, and expand it to a 2-dimensional system (with equations between proofs).

\todo{Elimination of the false proposition?}

\section{Predicative Higher-Order Propositional Logic with Extensional Equality}

We call the following type theory $\lambda o e$, or \emph{predicative higher-order propositional logic with extensional equality}.  

\input{PHOPL/Grammar.tex}
\input{PHOPL/PathSub.tex}
\input{PHOPL/Red.tex}
\input{PHOPL/Rules.tex}
\input{PHOPL/Meta.tex}
\input{PHOPL/KeyRedex2.tex}
\input{PHOPL/Computable.tex}
\input{PHOPL/SubC.tex}
\input{PHOPL/MainProp.tex}

%TODO Canonicity

% \section{$\lambda o i$}

% We further extend the system so that the equations are elements of $\Omega$.  This allows us, for example,
% to form propositions of the form $M =_A N \supset N =_A M$.

% The system $\lambda o i$ ($\lambda o$ with \emph{internal} equality) is defined as follows.  The
% syntax is formed by extending the grammar of $\lambda o$ with
% \[
% \begin{array}{lrcl}
% \text{Term} & M, \phi & ::= & \cdots \mid M =_A M \\
% \text{Proof} & \delta & ::= & \cdots \mid \reff{M} \mid \delta \supset^* \delta \mid \univ{\phi}{\phi}{\delta}{\delta} \mid \triplelambda^{MM} e : x =_A x . \delta \mid \delta_{MM} \delta\\
% & & & \quad \mid \delta =^*_A \delta \mid \delta^+ \mid \delta^-
% \end{array}
% \]

% Notice that we now tag the $\triplelambda$ proofs with two terms.

% The rules of deduction of $\lambda o i$ are those of Figures \ref{fig:lambdao} and \ref{fig:lambdaoe} with one modification and two additions.  The introduction rule for $\triplelambda$ is changed to %TODO Give it a name
% \[ \infer{\Gamma \vdash \triplelambda^{FG} e : x =_A y . \delta : F =_{A \rightarrow B} G}
% {\Gamma, x : A, y : A, e : x =_A y \vdash \delta : F x =_B G y} \]
% and we add the rules:
% \[ \infer{\Gamma \vdash M =_A N : \Omega}{\Gamma \vdash M : A \quad \Gamma \vdash N : A} \]
% \[ \infer{\Gamma \vdash \delta =^*_A \epsilon : (M =_A N) =_\Omega (M' =_A N')}
% {\Gamma \vdash \delta : M =_A M' \quad \Gamma \vdash \epsilon : N =_A N'} \]

% We extend the definition of path substitution by
% \[ (N =_B N') \{ \vec{x} := \vec{P} : \vec{M} \sim \vec{M'} \}
% \eqdef N \{ \vec{x} := \vec{P} : \vec{M} \sim \vec{M'} \} =_B^*
% N' \{ \vec{x} := \vec{P} : \vec{M} \sim \vec{M'} \} \enspace . \]

% We define terms $\sym{A}{M}{N}{\delta}$ and $\trans{A}{M}{N}{P}{\delta}{\epsilon}$.
% \begin{align*}
% \sym{\Omega}{\phi}{\psi}{\delta} & \eqdef \univ{\psi}{\phi}{\delta^-}{\delta^+} \\
% \sym{A \rightarrow B}{M}{N}{\delta} & \eqdef \triplelambda p:x =_A y. \sym{B}{My}{Nx}{\delta
% \sym{A}{x}{y}{p}} \\
% & \\
% \trans{\Omega}{\phi}{\psi}{\chi}{\delta}{\epsilon} & \eqdef \univ{\phi}{\chi}
% {\lambda p:\phi.\epsilon^+(\delta^+ p)}{\lambda p:\chi.\delta^-(\epsilon^- p)} \\
% \trans{A \rightarrow B}{M}{N}{P}{\delta}{\epsilon}
% & \eqdef \triplelambda p:x =_A y. \trans{B}{Mx}{Nx}{Py}{\delta_{xx} \reff{x}}{\epsilon_{xy} p}
% \end{align*}

% \begin{lm}
% $ $
% \begin{enumerate}
% \item
% If $\Gamma \vdash \delta : M =_A N$ then $\Gamma \vdash \sym{A}{M}{N}{\delta} : N =_A M$.
% \item
% If $\Gamma \vdash \delta : M =_A N$ and $\Gamma \vdash \epsilon : N =_A P$ then
% $\Gamma \vdash \trans{A}{M}{N}{P}{\delta}{\epsilon} : M =_A P$.
% \end{enumerate}
% \end{lm}

% \begin{proof}
% Straightforward.
% \end{proof}

% The reduction relation is that of $\lambda o e$ together with the following clauses:

% \begin{align*}
% & \reff{M} =^*_A \reff{N}  \\ & \qquad \rhd \reff{M =_A N} \\ \\
% & \reff{\phi} =^*_\Omega \univ{\psi}{\chi}{\delta}{\epsilon}  \\ & \qquad \rhd 
%   \mathsf{univ}_{\phi =_\Omega \psi,\phi =_\Omega \chi} \\
% &  \qquad \qquad \left( \lambda p:\phi =_\psi. \univ{\phi}{\chi}{\lambda q:\phi.\delta (p^+ q)}
%     {\lambda q : \chi. p^- (\epsilon q)}, \right. \\ 
% &  \qquad \qquad \left. \lambda p:\phi =_\Omega \chi. \univ{\phi}{\psi}{\lambda q:\phi. \epsilon (p^+ q)}
%     {\lambda q : \psi. p^- (\delta q)} \right) \\ \\
% & \univ{\phi}{\psi}{\delta}{\epsilon} =^*_\Omega \reff{\chi}  \\ & \qquad \rhd
%   \mathsf{univ}_{\phi =_\Omega \chi, \psi =_\Omega \chi} \\
% & \qquad \qquad   \left( \lambda p:\phi = \chi . \univ{\psi}{\chi}{\lambda q:\psi. p^+ (\epsilon q)}
%       {\lambda q:\chi. \delta (p^- q)}, \right. \\
% & \qquad \qquad   \left. \lambda p:\psi =_\Omega \chi. \univ{\phi}{\chi}{\lambda q:\phi. p^+ (\delta q)}
%       {\lambda q:\chi. \epsilon (p^- q)} \right) \\ \\
% & \univ{\phi}{\psi}{\delta}{\epsilon} =^*_\Omega \univ{\phi'}{\psi'}{\delta'}{\epsilon'}
%  \\ & \qquad \rhd
% \mathsf{univ}_{\phi =_\Omega \phi', \psi =_\Omega \psi'} \\
% & \qquad \qquad \left( \lambda p:\phi = \phi'. \univ{\psi}{\psi'}{\lambda q:\psi. \delta' (p^+ (\epsilon q))}{\lambda q:\psi' . \delta (p^-(\epsilon' q))}, \right. \\
% & \qquad \qquad \left. \lambda p:\psi=_\Omega \psi' . \univ{\phi}{\phi'}{\lambda q:\phi. \epsilon' (p^+ (\delta q))}{\lambda q:\phi' . \epsilon (p^- (\delta' q))} \right) \\ \\
% & \reff{F} =^*_{A \rightarrow B} \triplelambda^{G G'} q:x =_A y. P
%  \\ & \qquad \rhd
% \mathsf{univ}_{F =_{A \rightarrow B} G, F =_{A \rightarrow B} G'} \\
% & \qquad \qquad \left( \lambda p : F =_{A \rightarrow B} G. \triplelambda^{F G'} q : x =_A y. 
% \trans{B}{Fx}{Gx}{G'y}{p_{xx} \reff{x}}{P}, \right. \\
% & \qquad \qquad \lambda p : F =_{A \rightarrow B} G'. \triplelambda^{F G} q : x =_A y. \\
% & \qquad \qquad \left. \trans{B}{Fx}{G'y}{Gx}{p_{xy} q}{\sym{B}{Gx}{G'y}{P}} \right) \\ \\
% & \triplelambda^{F F'} p : x =_A y. P =^*_{A \rightarrow B} \reff{G}
%   \\ & \qquad \rhd
% \mathsf{univ}_{F =_{A \rightarrow B} G,F' =_{A \rightarrow B} G} \\
% & \qquad \qquad \left( \lambda q : F =_{A \rightarrow B} G .
% \triplelambda^{F' G} p : x =_A y. \right. \\
% & \qquad \qquad \trans{B}{F'x}{Fx}{Gy}{\sym{B}{Fx}{F'x}{P [ y := x, p := \reff{x} ] }}
% {
%  q_{xy}p}, \\
% & \qquad \qquad \left. \lambda q:F'=_{A \rightarrow B} G. \triplelambda^{FG} p : x =_A y.
% \trans{B}{Fx}{F'y}{Gy}{P}{q_{yy} \reff{y}} \right)
% \end{align*}

% \begin{align*}
% & (\triplelambda^{F F'} p : x =_A y. P) =^*_{A \rightarrow B} (\triplelambda^{G G'} p : x =_A y . Q)
%  \\ & \qquad \rhd 
% \mathsf{univ}_{F =_{A \rightarrow B} G,F' =_{A \rightarrow B} G'} \\
% & \qquad \qquad \left( \lambda q : F =_{A \rightarrow B} G . \triplelambda^{F' G'} p : x =_A y. \right. \\
% & \qquad \qquad \mathsf{trans}_{B,F'x,Fx,G'y} \left( \sym{B}{Fx}{F'x}{P [ y := x, p := \reff{x} ]} , \right. \\
% & \qquad \qquad \left. \trans{B}{Fx}{Gx}{G'y}{q_{xx} \reff{x}}{Q} \right) , \\
% & \qquad \qquad \lambda q : F' =_{A \rightarrow B} G' . \triplelambda^{FG} p : x =_A y. \\
% & \qquad \qquad \mathsf{trans}_{B, Fx, F'x, Gy} \left( P [ y := x,  p := \reff{x} ] , \right. \\
% & \qquad \qquad \! \! \left. \left. \trans{B}{F'x}{G'y}{Gy}{q_{xy} p}{\sym{B}{Gy}{G'y}{Q [ x := y, p := \reff{y} ] }} \right) \right)
% \end{align*}

% \subsection{Proof of Strong Normalisation}

% All the results of Section \ref{section:meta} hold for $\lambda o i$ as well,
% with very similar proofs.

% We define the sets of computable expressions $E_\Gamma(\phi)$ for propositions
% $\phi$ as in Definition \ref{df:computable}.  The only thing to bear in mind
% is that, in the definition of $E_\Gamma(\phi \supset \psi)$, the
% propositions $\phi$ and $\psi$ might now have the form $M =_A N$.  For completeness, we write out the definition here:

% \begin{align*}
% E_\Gamma(\Omega) \eqdef & \{ M \mid \Gamma \vdash M : \Omega, M \in \SN \} \\
% E_\Gamma(A \rightarrow B) \eqdef & \{ M \mid \Gamma \vdash M : A \rightarrow B, \\
% & \quad \forall (\Delta \supseteq \Gamma) (N \in E_\Delta(A)). MN \in E_\Delta(B), \\
% & \quad \forall (\Delta \supseteq \Gamma) (N, N' \in E_\Delta(A)) (\delta \in E_\Delta(N =_A N')). \\
% & \quad \quad \reff{M}_{N N'} \delta \in E_\Gamma(MN =_B MN') \} \\
% \\
% E_\Gamma(\bot) & \eqdef \{ \delta \mid \Gamma \vdash \delta : \bot, \delta \in \SN \} \\
% E_\Gamma(\phi \supset \psi) & \eqdef \{ \delta \mid \Gamma \vdash \delta : \phi \supset \psi, \\
% & \forall (\Delta \supseteq \Gamma)(\epsilon \in E_\Delta(\phi)). \delta \epsilon \in E_\Gamma(\psi) \} \\
% E_\Gamma(\phi =_\Omega \psi) & \eqdef \{ \delta \mid \Gamma \vdash \delta : \phi =_\Omega \psi, \\
% & \delta^+ \in E_\Gamma(\phi \supset \psi), \delta^- \in E_\Gamma(\psi \supset \phi) \} \\
% E_\Gamma(M =_{A \rightarrow B} M') & \eqdef \{ \delta \mid \Gamma \vdash \delta : M =_{A \rightarrow B} M', \\
% & \forall (\Delta \supseteq \Gamma) (N, N' \in E_\Delta(A)) (\epsilon \in E_\Delta(N =_A N')). \\
% & \delta_{NN'}\epsilon \in E_\Delta(MN =_B M'N') \} \\
% E_\Gamma(\phi) & \eqdef \{ \delta \mid \Gamma \vdash \delta : \phi, \delta \in \SN \} \\
% & \qquad (\phi \text{ neutral}) \\
% E_\Gamma(\phi) & \eqdef E_\Gamma(\nf{\phi}) \\
% & \qquad (\phi \mbox{ a normalizable term of type $\Omega$}) \\
% \end{align*}

% \begin{lemma}
% \label{lm:Ered}
% If $(\triplelambda p:x =_A y. \delta)_{M N} \epsilon \theta_1 \cdots \theta_n \in E_\Gamma(\phi)$
% then $\delta[x:=M, y:=N, p:=\epsilon] \theta_1 \cdots \theta_n \in E_\Gamma(\phi)$.
% \end{lemma}

% \begin{proof}
% The proof is by an induction on $\nf{\phi}$.
% \end{proof}

% \begin{lemma}
% \label{lm:eqstar}
% Let $M, M', N, N' \in E_\Gamma(A)$.
% If $\delta \in E_\Gamma(M =_A M')$ and $\epsilon \in E_\Gamma(N =_A N')$ then
% $\delta =_A^* \epsilon \in E_\Gamma((M =_A N) =_\Omega (M' =_A N'))$.
% \end{lemma}

% \begin{proof}
% We must prove that $(\delta =_A^* \epsilon)^+ \in E_\Gamma(M =_A N \supset M' =_A N')$ and
% $(\delta =_A^* \epsilon)^- \in E_\Gamma(M' =_A N' \supset M =_A N)$.  We prove the first of these; the proof of the second is similar.

% In fact, we prove the following statement, from which the desired conclusion easily follows:

% \begin{quote}
% Let $A \equiv A_1 \rightarrow \cdots \rightarrow A_n \rightarrow \Omega$ be a type.  Let
% \begin{align*}
% \delta & \in E_\Gamma(M =_A M') \\
% \epsilon & \in E_\Gamma(N =_A N') \\
% \chi & \in E_\Gamma(M =_A N) \\
% \theta_i & \in E_\Gamma(L_i =_{A_i} L_i') & (1 \leq i \leq n) \\
% \alpha & \in E_\Gamma(M L_1 \cdots L_n) \\
% N L_1' \cdots L_n' & \twoheadrightarrow_\beta \phi_1 \supset \cdots \supset \phi_m \supset \bot \\
% \beta_j & \in E_\Gamma(\phi_j) & (1 \leq j \leq m)
% \end{align*}
% Then $((\delta =_A^* \epsilon)^+ \chi_{L_1 L_1'} \theta_1 \cdots_{L_n L_n'} \theta_n)^+ \alpha \beta_1 \cdots \beta_m \in \SN$.
% \end{quote}

% The proof is by induction on the fact that $\delta, \epsilon, \chi, \theta_i, \alpha, \beta_j \in \SN$.

% Consider a possible one-step reduction from $((\delta =_A^* \epsilon)^+ \chi \vec{\theta})^+ \alpha \vec{\beta}$.  If the reduction consists of reducing one of the subterms, we apply the induction hypothesis.  The only other possibility is that $\delta =_A^* \epsilon$ is a redex.  There are now seven cases to consider: we give the details for one of them.

% Let $\delta \equiv \triplelambda^{F F'} p : x =_{A_1} y.P$ and $\epsilon \equiv \triplelambda^{G G'} p : x =_{A_1} y. Q$.  We must prove that
% \begin{align*} & \mathsf{univ}_{F =_{A \rightarrow B} G,F' =_{A \rightarrow B} G'} \\
% & \qquad \qquad \left( \lambda q : F =_{A \rightarrow B} G . \triplelambda p : x =_A y. \right. \\
% & \qquad \qquad \mathsf{trans}_{A_2 \rightarrow \cdots \rightarrow A_n \rightarrow B} \left( \sym*{P [ y := x, p := \reff{x} ]} , \right. \\
% & \qquad \qquad \left. \trans*{q_{xx} \reff{x}}{Q} \right) , \\
% & \qquad \qquad \lambda q : F' =_{A \rightarrow B} G' . \triplelambda p : x =_A y. \\
% & \qquad \qquad \mathsf{trans} \left( P [ y := x,  p := \reff{x} ] , \right. \\
% & \qquad \qquad \! \! \left. \left. \trans*{q_{xy} p}{\sym*{Q [ x := y, p := \reff{y} ] }} \right) \right)^+ \chi \vec{\theta})^+ \alpha \vec{\beta} \in \SN \end{align*}
% By Lemma \ref{lm:wte_loi1}, it is sufficient to prove that
% \begin{align*} & ( \left( \lambda q : F =_{A \rightarrow \Omega} G . \triplelambda p : x =_A y. \right. \\
% & \qquad \qquad \mathsf{trans}_{A_2 \rightarrow \cdots \rightarrow A_n \rightarrow \Omega} \left( P[y:=x, p:=\reff{x}] , \right. \\
% & \qquad \qquad \left. \trans*{q_{xx} \reff{x}}{Q} \right) \chi \vec{\theta})^+ \alpha \vec{\beta} \in \SN \end{align*} 
% By Lemma \ref{lm:wte_loi2}, it is sufficient to prove that
% \begin{align*} & ( \left( \triplelambda p : x =_A y. \right. \\
% & \qquad \qquad \mathsf{trans}_{A_2 \rightarrow \cdots \rightarrow A_n \rightarrow \Omega} \left( P[y:=x, p:=\reff{x}] , \right. \\
% & \qquad \qquad \left. \trans*{\chi_{xx} \reff{x}}{Q} \right) \vec{\theta})^+ \alpha \vec{\beta} \in \SN \end{align*} 
% By Lemma \ref{lm:wte_loi3}, it is sufficient to prove that
% \begin{align*}
% & \qquad \qquad (\mathsf{trans}_{A_2 \rightarrow \cdots \rightarrow A_n \rightarrow \Omega} \left( P[x:=L_1, y:=L_1, p:=\reff{L_1}] , \right. \\
% & \qquad \qquad \left. \trans*{\chi_{L_1 L_1} \reff{L_1}}{Q[x:=L_1, y:=L_1', p:=\theta_1]} \right) \theta_2 \cdots \theta_n)^+ \alpha \vec{\beta} \in \SN \end{align*}
% Repeatedly applying Lemma \ref{lm:wte_loi3}, it is sufficient to prove that
% \begin{align*}
% & \qquad \qquad (\mathsf{trans}_\Omega \left( P[x:=L_1, y:=L_1, p:=\reff{L_1}]_{L_2 L_2} \reff{L_2} \cdots_{L_n L_n} \reff{L_n} , \right. \\
% & \qquad \qquad \left. \trans*{\chi_{L_1 L_1} \reff{L_1}}{Q[x:=L_1, y:=L_1', p:=\theta_1]}_{L_2 L_2'} \theta_2 \cdots_{L_n L_n'} \theta_n \right) )^+ \alpha \vec{\beta} \in \SN \end{align*}
%  By Lemma \ref{lm:wte_loi1}, it is sufficient to prove that
% \begin{align*}
% & (\lambda p. (\trans*{\chi_{L_1 L_1} \reff{L_1}}{Q[x:=L_1, y:=L_1', p:=\theta_1]}_{L_2 L_2'} \theta_2 \cdots_{L_n L_n'} \theta_n)^+ \\
% & \quad ((P[x:=L_1, y:=L_1, p:=\reff{L_1}]_{L_2 L_2} \reff{L_2} \cdots_{L_n L_n} \reff{L_n})^+ p)) \alpha \vec{\beta} \in \SN
% \end{align*}
% and
% \begin{align*}
% & \lambda p. (P[x:=L_1, y:=L_1, p:=\reff{L_1}]_{L_2 L_2} \reff{L_2} \cdots_{L_n L_n} \reff{L_n})^- \\
% & \quad ((\trans*{\chi_{L_1 L_1} \reff{L_1}}{Q[x:=L_1, y:=L_1', p:=\theta_1]}_{L_2 L_2'} \theta_2 \cdots_{L_n L_n'} \theta_n)^- p) \in \SN
% \end{align*}

% We prove the first of these here.
% By Lemma \ref{lm:wte_loi2}, it is sufficient to prove that
% \begin{align*}
% & (\trans*{\chi_{L_1 L_1} \reff{L_1}}{Q[x:=L_1, y:=L_1', p:=\theta_1]}_{L_2 L_2'} \theta_2 \cdots_{L_n L_n'} \theta_n)^+ \\
% & \quad ((P[x:=L_1, y:=L_1, p:=\reff{L_1}]_{L_2 L_2} \reff{L_2} \cdots_{L_n L_n} \reff{L_n})^+ \alpha) \vec{\beta} \in \SN
% \end{align*}
% Repeatedly appling the three lemmas again, it is sufficient to prove that
% \begin{align*}
% & (Q [x:= L_1, y := L_1', p:=\theta_1] \vec{\theta})^+ ((\chi \reff{L_1} \cdots
% \reff{L_n})^+ \\
% & \quad ((P[x:=L_1, y:=L_1, p:=\reff{L_1}]_{L_2 L_2} \reff{L_2} \cdots_{L_n L_n} \reff{L_n})^+ \alpha)) \vec{\beta} \in \SN
% \end{align*}

% Now, we have $\delta \in E_\Gamma(M =_A M')$, hence $\delta_{L_1L_1} \reff{L_1}
% \in E_\Gamma(M L_1 = M' L_1)$ and so $P[x := L_1, y := L_1, p := \reff{L_1}]
% \in E_\Gamma(M L_1 = M' L_1)$ by Lemma \ref{lm:Ered}.  Similarly
% $Q[x:=L_1, y:=L_1', p:=\theta_1] \in E_\Gamma(N L_1 = N' L_1')$.  The
% result follows.
% \end{proof}

% We define what it means to be a computable substitution and a computable path substitution as before.

% \begin{theorem}
% $ $
% \begin{enumerate}
% \item
% If $\Gamma \vdash M : A$, and $\sigma : \Gamma \rightarrow \Delta$ is computable,
% then $M [ \sigma ] \in E_\Delta(A)$.
% \item
% If $\Gamma \vdash \delta : \phi$, and $\sigma : \Gamma \rightarrow \Delta$ is computable,
% then $\delta [ \sigma ] \in E_\Delta(\phi[\sigma])$.
% \item
% If $\Gamma \vdash P : M =_A N$, and $\sigma : \Gamma \rightarrow \Delta$ is computable,
% then $P [ \sigma ] \in E_\Delta(M [ \sigma ] =_A N [ \sigma ])$.
% \item
% If $\Gamma \vdash M : A$, $\tau : \sigma \sim \rho : \Gamma \rightarrow \Delta$, and $\tau$, $\sigma$
% and $\rho$ are all computable, then $M \{ \tau : \sigma \sim \rho \} \in E_\Delta(M [ \sigma ] =_A M [ \rho ])$.
% \end{enumerate}
% \end{theorem}

% \begin{proof}
% Induction on derivations, as before.  We use Lemma \ref{lm:eqstar} for the rule
% $(=^*)$.
% \end{proof}

\section{Future Work}

We have shown that it is possible, in a system with non-dependent function types and implication, to give a strongly normalizing,
confluent reduction rule for the univalence constructor.  We now intend to do the same for stronger and stronger systems, getting
ever closer to full homotopy type theory.  The next steps will be:

\begin{itemize}
\item
a system where the equations $M =_A N$ are objects of $\Omega$, allowing us to form propositions such as $M =_A N \supset N =_A M$.
\item
a system with universal quantification over the types $A$, allowing us to form propositions such as $\forall x:A. x =_A x$ and
$\forall x,y : A. x =_A y \supset y =_A x$
\end{itemize}

\todos

\begin{frame}
\frametitle{Bibliography}
\bibliography{type}
\end{frame}

% \appendix

% \section{About the Formalization}

% \input{Prelims.tex}
% \mode<all>{\input{Grammar/Taxonomy.tex}}
% \mode<all>{\input{Grammar/Base.tex}}

% We define the operations of replacement and substitution on
% expressions.  

% \input{Grammar/Substitution/PreOpFamily.tex}
% \input{Grammar/Substitution/OpFamily.tex}

% The details are given in Appendix \ref{appendix:repsub}.

% \input{Grammar/Context.tex}
% \input{Reduction/Base.tex}
% \input{Reduction/SN.tex}
% %\input{PL/Grammar.tex}
% %\input{PL/Rules.tex}
% %\input{PL/Computable.tex}

% \section{Replacement and Substitution}
% \label{appendix:repsub}

% \input{Grammar/OpFamily/PreOpFamily.tex}
% \input{Grammar/OpFamily/Lifting.tex}
% \input{Grammar/OpFamily/LiftFamily.tex}
% \input{Grammar/OpFamily/Composition.tex}
% \input{Grammar/OpFamily/OpFamily.tex}
% \input{Grammar/Replacement.tex}
% \input{Grammar/Substitution/Lifting.tex}
% \input{Grammar/Substitution/RepSub.tex}
% \input{Grammar/Substitution/LiftFamily.tex}
% \input{Grammar/Substitution/Botsub.tex}

\end{document}
