\AgdaHide{
\begin{code}%
\>\AgdaKeyword{module} \AgdaModule{PHOPL.MainProp} \AgdaKeyword{where}\<%
\\
\>\AgdaKeyword{open} \AgdaKeyword{import} \AgdaModule{Data.Empty} \AgdaKeyword{renaming} \AgdaSymbol{(}\AgdaDatatype{⊥} \AgdaSymbol{to} \AgdaDatatype{Empty}\AgdaSymbol{)}\<%
\\
\>\AgdaKeyword{open} \AgdaKeyword{import} \AgdaModule{Data.Unit}\<%
\\
\>\AgdaKeyword{open} \AgdaKeyword{import} \AgdaModule{Data.Product} \AgdaKeyword{renaming} \AgdaSymbol{(}\AgdaInductiveConstructor{\_,\_} \AgdaSymbol{to} \AgdaInductiveConstructor{\_,p\_}\AgdaSymbol{)}\<%
\\
\>\AgdaKeyword{open} \AgdaKeyword{import} \AgdaModule{Data.List}\<%
\\
\>\AgdaKeyword{open} \AgdaKeyword{import} \AgdaModule{Prelims}\<%
\\
\>\AgdaKeyword{open} \AgdaKeyword{import} \AgdaModule{PHOPL.Grammar}\<%
\\
\>\AgdaKeyword{open} \AgdaKeyword{import} \AgdaModule{PHOPL.Rules}\<%
\\
\>\AgdaKeyword{open} \AgdaKeyword{import} \AgdaModule{PHOPL.PathSub}\<%
\\
\>\AgdaKeyword{open} \AgdaKeyword{import} \AgdaModule{PHOPL.Red}\<%
\\
\>\AgdaKeyword{open} \AgdaKeyword{import} \AgdaModule{PHOPL.Neutral}\<%
\\
\>\AgdaKeyword{open} \AgdaKeyword{import} \AgdaModule{PHOPL.Meta}\<%
\\
\>\AgdaKeyword{open} \AgdaKeyword{import} \AgdaModule{PHOPL.Computable}\<%
\\
\>\AgdaKeyword{open} \AgdaKeyword{import} \AgdaModule{PHOPL.SubC}\<%
\\
\>\AgdaKeyword{open} \AgdaKeyword{import} \AgdaModule{PHOPL.SN}\<%
\\
\>\AgdaKeyword{open} \AgdaKeyword{import} \AgdaModule{PHOPL.MainPropFinal}\<%
\\
\>\AgdaKeyword{open} \AgdaKeyword{import} \AgdaModule{PHOPL.MainProp1}\<%
\end{code}
}

Our main theorem is as follows.

\begin{theorem}$ $
\begin{enumerate}
\item
If $\Gamma \vdash M : A$, and $\sigma : \Gamma \rightarrow \Delta$ is computable,
then $M [ \sigma ] \in E_\Delta(A)$.
\item
If $\Gamma \vdash \delta : \phi$, and $\sigma : \Gamma \rightarrow \Delta$ is computable,
then $\delta [ \sigma ] \in E_\Delta(\phi[\sigma])$.
\item
If $\Gamma \vdash P : M =_A N$, and $\sigma : \Gamma \rightarrow \Delta$ is computable,
then $P [ \sigma ] \in E_\Delta(M [ \sigma ] =_A N [ \sigma ])$.
\item
\label{computable-path-sub}
If $\Gamma \vdash M : A$, $\tau : \sigma \sim \rho : \Gamma \rightarrow \Delta$, and $\tau$, $\sigma$
and $\rho$ are all computable, then $M \{ \tau : \sigma \sim \rho \} \in E_\Delta(M [ \sigma ] =_A M [ \rho ])$.
\end{enumerate}
\end{theorem}

\begin{code}%
\>\AgdaKeyword{postulate} \AgdaPostulate{Computable-Sub} \AgdaSymbol{:} \AgdaSymbol{∀} \AgdaSymbol{\{}\AgdaBound{U}\AgdaSymbol{\}} \AgdaSymbol{\{}\AgdaBound{V}\AgdaSymbol{\}} \AgdaSymbol{\{}\AgdaBound{K}\AgdaSymbol{\}} \AgdaSymbol{(}\AgdaBound{σ} \AgdaSymbol{:} \AgdaFunction{Sub} \AgdaBound{U} \AgdaBound{V}\AgdaSymbol{)} \AgdaSymbol{\{}\AgdaBound{Γ}\AgdaSymbol{\}} \AgdaSymbol{\{}\AgdaBound{Δ}\AgdaSymbol{\}} \<[63]%
\>[63]\<%
\\
\>[0]\AgdaIndent{25}{}\<[25]%
\>[25]\AgdaSymbol{\{}\AgdaBound{M} \AgdaSymbol{:} \AgdaFunction{Expression} \AgdaBound{U} \AgdaSymbol{(}\AgdaInductiveConstructor{varKind} \AgdaBound{K}\AgdaSymbol{)\}} \AgdaSymbol{\{}\AgdaBound{A}\AgdaSymbol{\}} \AgdaSymbol{→}\<%
\\
\>[0]\AgdaIndent{25}{}\<[25]%
\>[25]\AgdaBound{σ} \AgdaFunction{∶} \AgdaBound{Γ} \AgdaFunction{⇒C} \AgdaBound{Δ} \AgdaSymbol{→} \AgdaBound{Γ} \AgdaDatatype{⊢} \AgdaBound{M} \AgdaDatatype{∶} \AgdaBound{A} \AgdaSymbol{→} \AgdaDatatype{valid} \AgdaBound{Δ} \AgdaSymbol{→} \AgdaRecord{E'} \AgdaBound{Δ} \AgdaSymbol{(}\AgdaBound{A} \AgdaFunction{⟦} \AgdaBound{σ} \AgdaFunction{⟧}\AgdaSymbol{)} \AgdaSymbol{(}\AgdaBound{M} \AgdaFunction{⟦} \AgdaBound{σ} \AgdaFunction{⟧}\AgdaSymbol{)}\<%
\\
%
\\
\>\AgdaKeyword{postulate} \AgdaPostulate{Computable-Path-Substitution} \AgdaSymbol{:} \AgdaSymbol{∀} \AgdaBound{U} \AgdaBound{V} \AgdaSymbol{(}\AgdaBound{τ} \AgdaSymbol{:} \AgdaFunction{PathSub} \AgdaBound{U} \AgdaBound{V}\AgdaSymbol{)} \AgdaBound{σ} \AgdaBound{σ'} \AgdaBound{Γ} \AgdaBound{Δ} \AgdaBound{M} \AgdaBound{A} \AgdaSymbol{→} \AgdaBound{σ} \AgdaFunction{∶} \AgdaBound{Γ} \AgdaFunction{⇒C} \AgdaBound{Δ} \AgdaSymbol{→} \AgdaBound{σ'} \AgdaFunction{∶} \AgdaBound{Γ} \AgdaFunction{⇒C} \AgdaBound{Δ} \AgdaSymbol{→} \AgdaBound{τ} \AgdaFunction{∶} \AgdaBound{σ} \AgdaFunction{∼} \AgdaBound{σ'} \AgdaFunction{∶} \AgdaBound{Γ} \AgdaFunction{⇒C} \AgdaBound{Δ} \AgdaSymbol{→} \AgdaBound{Γ} \AgdaDatatype{⊢} \AgdaBound{M} \AgdaDatatype{∶} \AgdaBound{A} \AgdaSymbol{→} \AgdaDatatype{valid} \AgdaBound{Δ} \AgdaSymbol{→} \<[151]%
\>[151]\<%
\\
\>[25]\AgdaIndent{39}{}\<[39]%
\>[39]\AgdaFunction{EE} \AgdaBound{Δ} \AgdaSymbol{(}\AgdaBound{M} \AgdaFunction{⟦} \AgdaBound{σ} \AgdaFunction{⟧} \AgdaFunction{≡〈} \AgdaFunction{yt} \AgdaBound{A} \AgdaFunction{〉} \AgdaBound{M} \AgdaFunction{⟦} \AgdaBound{σ'} \AgdaFunction{⟧}\AgdaSymbol{)} \AgdaSymbol{(}\AgdaBound{M} \AgdaFunction{⟦⟦} \AgdaBound{τ} \AgdaFunction{∶} \AgdaBound{σ} \AgdaFunction{∼} \AgdaBound{σ'} \AgdaFunction{⟧⟧}\AgdaSymbol{)} \<%
\end{code}

\AgdaHide{
\begin{code}%
\>\AgdaComment{\{-Computable-Sub σ σ∶Γ⇒Δ (varR x validΓ) validΔ = σ∶Γ⇒Δ x\<\\
\>Computable-Sub \{V = V\} σ \{Δ = Δ\} σ∶Γ⇒Δ (appR Γ⊢M∶A⇛B Γ⊢N∶A) validΔ = \<\\
\>  appT-E validΔ (Computable-Sub σ σ∶Γ⇒Δ Γ⊢M∶A⇛B validΔ) (Computable-Sub σ σ∶Γ⇒Δ Γ⊢N∶A validΔ)\<\\
\>Computable-Sub σ σ∶Γ⇒Δ (ΛR \{M = M\} \{B\} Γ,A⊢M∶B) validΔ = \<\\
\>  func-E (λ \_ Θ ρ N validΘ ρ∶Δ⇒Θ N∈EΘA → \<\\
\>    let MN∈EΘB = subst (E Θ B) (subrepsub M)\<\\
\>                 (Computable-Sub (x₀:= N •SR Rep↑ \_ ρ • Sub↑ -Term σ) \<\\
\>                 (compC (compSRC (botsubC N∈EΘA) \<\\
\>                        (Rep↑-typed ρ∶Δ⇒Θ)) \<\\
\>                 (Sub↑C σ∶Γ⇒Δ)) \<\\
\>                 Γ,A⊢M∶B validΘ) in\<\\
\>    expand-E MN∈EΘB\<\\
\>      (appR (ΛR (Weakening (Substitution Γ,A⊢M∶B (ctxTR validΔ) (Sub↑-typed (subC-typed σ∶Γ⇒Δ))) \<\\
\>                                                      (ctxTR validΘ) \<\\
\>                                         (Rep↑-typed ρ∶Δ⇒Θ))) \<\\
\>                (E-typed N∈EΘA)) \<\\
\>      (βTkr (SNap' \{Ops = substitution\} R-respects-sub (E-SN B MN∈EΘB))))\<\\
\>Computable-Sub σ σ∶Γ⇒Δ (⊥R \_) validΔ = ⊥-E validΔ\<\\
\>Computable-Sub σ σ∶Γ⇒Δ (⊃R Γ⊢φ∶Ω Γ⊢ψ∶Ω) validΔ = ⊃-E \<\\
\>  (Computable-Sub σ σ∶Γ⇒Δ Γ⊢φ∶Ω validΔ) (Computable-Sub σ σ∶Γ⇒Δ Γ⊢ψ∶Ω validΔ)\<\\
\>Computable-Sub σ σ∶Γ⇒Δ (appPR Γ⊢δ∶φ⊃ψ Γ⊢ε∶φ) validΔ = appP-EP \<\\
\>  (Computable-Sub σ σ∶Γ⇒Δ Γ⊢δ∶φ⊃ψ validΔ) (Computable-Sub σ σ∶Γ⇒Δ Γ⊢ε∶φ validΔ)\<\\
\>Computable-Sub σ \{Γ = Γ\} \{Δ = Δ\} σ∶Γ⇒Δ (ΛPR \{δ = δ\} \{φ\} \{ψ\} Γ⊢φ∶Ω Γ,φ⊢δ∶ψ) validΔ = \<\\
\>  let Δ⊢Λφδσ∶φ⊃ψ : Δ ⊢ (ΛP φ δ) ⟦ σ ⟧ ∶ φ ⟦ σ ⟧ ⊃ ψ ⟦ σ ⟧\<\\
\>      Δ⊢Λφδσ∶φ⊃ψ = Substitution \{A = φ ⊃ ψ\} (ΛPR Γ⊢φ∶Ω Γ,φ⊢δ∶ψ) validΔ (subC-typed σ∶Γ⇒Δ) in\<\\
\>  func-EP (λ W Θ ρ ε ρ∶Δ⇒Θ ε∈EΔφ → \<\\
\>    let δε∈EΘψ : EP Θ (ψ ⟦ σ ⟧ 〈 ρ 〉) (δ ⟦ Sub↑ \_ σ ⟧ 〈 Rep↑ \_ ρ 〉 ⟦ x₀:= ε ⟧)\<\\
\>        δε∈EΘψ = subst₂ (EP Θ) (subrepbotsub-up ψ) (subrepsub δ) \<\\
\>                 (Computable-Sub (x₀:= ε •SR Rep↑ \_ ρ • Sub↑ \_ σ) \<\\
\>                 (compC (compSRC (botsubCP ε∈EΔφ) \<\\
\>                        (Rep↑-typed ρ∶Δ⇒Θ)) \<\\
\>                 (Sub↑C σ∶Γ⇒Δ)) Γ,φ⊢δ∶ψ (Context-Validity (EP-typed ε∈EΔφ))) in\<\\
\>    expand-EP δε∈EΘψ (appPR (Weakening Δ⊢Λφδσ∶φ⊃ψ (Context-Validity (EP-typed ε∈EΔφ)) ρ∶Δ⇒Θ) (EP-typed ε∈EΔφ))\<\\
\>      (βPkr (SNrep R-creates-rep (E-SN Ω (Computable-Sub σ σ∶Γ⇒Δ Γ⊢φ∶Ω validΔ))) (EP-SN ε∈EΔφ))) \<\\
\>  Δ⊢Λφδσ∶φ⊃ψ\<\\
\>Computable-Sub σ σ∶Γ⇒Δ (convR Γ⊢δ∶φ Γ⊢ψ∶Ω φ≃ψ) validΔ = conv-E' (respects-conv (respects-osr substitution R-respects-sub) φ≃ψ) \<\\
\>  (Computable-Sub σ σ∶Γ⇒Δ Γ⊢δ∶φ validΔ) (ctxPR (Substitution Γ⊢ψ∶Ω validΔ (subC-typed σ∶Γ⇒Δ)))\<\\
\>Computable-Sub σ σ∶Γ⇒Δ (refR Γ⊢M∶A) validΔ = ref-EE (Computable-Sub σ σ∶Γ⇒Δ Γ⊢M∶A validΔ)\<\\
\>Computable-Sub σ σ∶Γ⇒Δ (⊃*R Γ⊢φ∶Ω Γ⊢ψ∶Ω) validΔ = ⊃*-EE (Computable-Sub σ σ∶Γ⇒Δ Γ⊢φ∶Ω validΔ) (Computable-Sub σ σ∶Γ⇒Δ Γ⊢ψ∶Ω validΔ)\<\\
\>Computable-Sub σ σ∶Γ⇒Δ (univR Γ⊢δ∶φ⊃ψ Γ⊢ε∶ψ⊃φ) validΔ = univ-EE (Computable-Sub σ σ∶Γ⇒Δ Γ⊢δ∶φ⊃ψ validΔ) (Computable-Sub σ σ∶Γ⇒Δ Γ⊢ε∶ψ⊃φ validΔ)\<\\
\>Computable-Sub σ σ∶Γ⇒Δ (plusR Γ⊢P∶φ≡ψ) validΔ = plus-EP (Computable-Sub σ σ∶Γ⇒Δ Γ⊢P∶φ≡ψ validΔ)\<\\
\>Computable-Sub σ σ∶Γ⇒Δ (minusR Γ⊢P∶φ≡ψ) validΔ = minus-EP (Computable-Sub σ σ∶Γ⇒Δ Γ⊢P∶φ≡ψ validΔ)\<\\
\>Computable-Sub σ σ∶Γ⇒Δ (lllR Γ⊢M∶A) validΔ = \{!!\}\<\\
\>Computable-Sub σ σ∶Γ⇒Δ (app*R Γ⊢M∶A Γ⊢M∶A₁ Γ⊢M∶A₂ Γ⊢M∶A₃) validΔ = \{!!\}\<\\
\>Computable-Sub σ σ∶Γ⇒Δ (convER Γ⊢M∶A Γ⊢M∶A₁ Γ⊢M∶A₂ M≃M' N≃N') validΔ = \{!!\}\<\\
\>\<\\
\>--TODO Rename\<\\
\>Computable-Path-Substitution U V τ σ σ' Γ Δ .(var x) .\_ σ∶Γ⇒CΔ σ'∶Γ⇒CΔ τ∶σ∼σ' (varR x \_) \_ = \<\\
\>  τ∶σ∼σ' x\<\\
\>Computable-Path-Substitution U V τ σ σ' Γ Δ .(app -bot out) .(ty Ω) σ∶Γ⇒CΔ σ'∶Γ⇒CΔ τ∶σ∼σ' (⊥R x) validΔ = ref-EE (⊥-E validΔ)\<\\
\>Computable-Path-Substitution U V τ σ σ' Γ Δ \_ .(ty Ω) σ∶Γ⇒CΔ σ'∶Γ⇒CΔ τ∶σ∼σ' (⊃R Γ⊢φ∶Ω Γ⊢ψ∶Ω) validΔ = ⊃*-EE \<\\
\>  (Computable-Path-Substitution U V τ σ σ' Γ Δ \_ (ty Ω) σ∶Γ⇒CΔ σ'∶Γ⇒CΔ τ∶σ∼σ' Γ⊢φ∶Ω validΔ) \<\\
\>  (Computable-Path-Substitution U V τ σ σ' Γ Δ \_ (ty Ω) σ∶Γ⇒CΔ σ'∶Γ⇒CΔ τ∶σ∼σ' Γ⊢ψ∶Ω validΔ) \<\\
\>Computable-Path-Substitution U V τ σ σ' Γ Δ \_ .(ty B) σ∶Γ⇒CΔ σ'∶Γ⇒CΔ τ∶σ∼σ' (appR \{N = N\} \{A\} \{B\} Γ⊢M∶A⇒B Γ⊢N∶A) validΔ = \<\\
\>  app*-EE \<\\
\>  (Computable-Path-Substitution U V τ σ σ' Γ Δ \_ \_ σ∶Γ⇒CΔ σ'∶Γ⇒CΔ τ∶σ∼σ' Γ⊢M∶A⇒B validΔ) \<\\
\>  (Computable-Path-Substitution U V τ σ σ' Γ Δ \_ \_ σ∶Γ⇒CΔ σ'∶Γ⇒CΔ τ∶σ∼σ' Γ⊢N∶A validΔ)\<\\
\>  (Computable-Substitution U V σ Γ Δ N A (pathsubC-valid₁ \{U\} \{V\} \{τ\} \{σ\} \{σ'\} τ∶σ∼σ') Γ⊢N∶A refl validΔ)\<\\
\>  (Computable-Substitution U V σ' Γ Δ N A (pathsubC-valid₂ \{τ = τ\} \{σ\} \{σ = σ'\} \{Γ\} \{Δ\} τ∶σ∼σ') Γ⊢N∶A refl validΔ)-\}}\<%
\end{code}
}

\begin{proof}
The four parts are proved simultaneously by induction on derivations.  We give the details of
one case here, for part \ref{computable-path-sub} for the rule
\[ \infer{\Gamma \vdash \lambda x:A.M : A \rightarrow B}{\Gamma, x : A \vdash M : B} \]

We must prove that 
\[ \triplelambda e:a =_A a' . M \{ \tau : \sigma \sim \rho, x := e : a \sim a' \} \in E_\Delta(\lambda x:A.M[\sigma] =_{A \rightarrow B} \lambda x:A.M[\rho]) \enspace . \]
So let $\Theta \supseteq \Delta$; $N, N' \in E_\Theta(A)$; and $Q \in E_\Theta(N =_A N')$.  The induction hypothesis gives
\[ M \{ \tau , x := Q \} \in E_\Theta(M[\sigma, x:= N] =_B M [ \rho, x := N' ]) \enspace . \]
Applying Lemmas \ref{lm:expand-compute} and \ref{lm:conv-compute} gives
\[ (\triplelambda e:a =_A a' . M \{ \tau, x := e \})_{N N'} Q \in E_\Theta((\lambda x:A.M[\sigma]) N =_B (\lambda x:A.M[\rho]) N') \]
as required.
\end{proof}

\AgdaHide{
\begin{code}%
\>\AgdaComment{\{-Computable-Path-Substitution .U V τ σ σ' .Γ Δ \_ \_ σ∶Γ⇒CΔ σ'∶Γ⇒CΔ τ∶σ∼σ' (ΛR \{U\} \{Γ\} \{A\} \{M\} \{B\} Γ,A⊢M∶B) validΔ = \<\\
\>  let validΔAA : valid (Δ ,T A ,T A)\<\\
\>      validΔAA = ctxTR (ctxTR validΔ) in\<\\
\>  let validΔAAE : valid (addpath Δ A)\<\\
\>      validΔAAE = ctxER (varR x₁ validΔAA) (varR x₀ validΔAA) in\<\\
\>  let σ∶Γ⇒Δ = subC-typed σ∶Γ⇒CΔ in\<\\
\>  let σ'∶Γ⇒Δ = subC-typed σ'∶Γ⇒CΔ in\<\\
\>  let sub↖σ-typed : sub↖ σ ∶ Γ ,T A ⇒ addpath Δ A\<\\
\>      sub↖σ-typed = sub↖-typed σ∶Γ⇒Δ in\<\\
\>  let sub↗σ'-typed : sub↗ σ' ∶ Γ ,T A ⇒ addpath Δ A\<\\
\>      sub↗σ'-typed = sub↗-typed σ'∶Γ⇒Δ in\<\\
\>  func-EE (lllR (convER (Path-Substitution Γ,A⊢M∶B\<\\
\>                             (pathsub↑-typed (pathsubC-typed \{τ = τ\} \{σ\} \{σ = σ'\} \{Γ\} \{Δ\} τ∶σ∼σ')) sub↖σ-typed sub↗σ'-typed\<\\
\>                             validΔAAE)\<\\
\>                             (appR (ΛR (Weakening \{ρ = Rep↑ \_ upRep\}\<\\
\>                                           \{M = ((M ⟦ Sub↑ \_ σ ⟧) 〈 Rep↑ \_ upRep 〉) 〈 Rep↑ \_ upRep 〉\} \<\\
\>                                        (Weakening \{ρ = Rep↑ \_ upRep\}\<\\
\>                                           \{M = (M ⟦ Sub↑ \_ σ ⟧) 〈 Rep↑ \_ upRep 〉\} \<\\
\>                                        (Weakening \{ρ = Rep↑ \_ upRep\} \{M = M ⟦ Sub↑ \_ σ ⟧\} \<\\
\>                                        (Substitution \{σ = Sub↑ -Term σ\} \{M = M\} Γ,A⊢M∶B (ctxTR validΔ) \<\\
\>                                          (Sub↑-typed (subC-typed σ∶Γ⇒CΔ))) (ctxTR (ctxTR validΔ)) (Rep↑-typed upRep-typed)) \<\\
\>                                        (ctxTR (ctxTR (ctxTR validΔ))) \<\\
\>                                        (Rep↑-typed upRep-typed)) \<\\
\>                           (ctxTR (ctxER (varR (↑ x₀) (ctxTR (ctxTR validΔ))) (varR x₀ (ctxTR (ctxTR validΔ))))) \<\\
\>                           (Rep↑-typed upRep-typed))) \<\\
\>                           (varR x₂ (ctxER ((varR (↑ x₀) (ctxTR (ctxTR validΔ)))) (varR x₀ (ctxTR (ctxTR validΔ))))))  \<\\
\>                              (let stepA : addpath Δ A ,T A ⊢ M ⟦ Sub↑ \_ σ' ⟧ 〈 Rep↑ \_ upRep 〉 〈 Rep↑ \_ upRep 〉 〈 Rep↑ \_ upRep 〉 ∶ ty B\<\\
\>                                   stepA = Weakening \{U = V , -Term , -Term , -Term\} \{V = V , -Term , -Term , -Path , -Term\} \{ρ = Rep↑ \_ upRep\} \{Γ = Δ , ty A , ty A , ty A\} \{M = M ⟦ Sub↑ \_ σ' ⟧ 〈 Rep↑ \_ upRep 〉 〈 Rep↑ \_ upRep 〉\} \<\\
\>                                      (Weakening \{ρ = Rep↑ \_ upRep\} \{Γ = Δ , ty A , ty A\}\<\\
\>                                         \{M = (M ⟦ Sub↑ \_ σ' ⟧) 〈 Rep↑ \_ upRep 〉\} \<\\
\>                                      (Weakening \{ρ = Rep↑ \_ upRep\} \{M = M ⟦ Sub↑ \_ σ' ⟧\} \<\\
\>                                      (Substitution \{σ = Sub↑ \_ σ'\} \{M = M\} \<\\
\>                                      Γ,A⊢M∶B \<\\
\>                                      (ctxTR validΔ) \<\\
\>                                      (Sub↑-typed σ'∶Γ⇒Δ))\<\\
\>                                      validΔAA \<\\
\>                                      (Rep↑-typed upRep-typed)) \<\\
\>                                      (ctxTR validΔAA) \<\\
\>                                      (Rep↑-typed upRep-typed))\<\\
\>                                      (ctxTR validΔAAE)\<\\
\>                                      (Rep↑-typed upRep-typed) in\<\\
\>                              let stepB : addpath Δ A ⊢ (ΛT A M) ⟦ σ' ⟧ ⇑ ⇑ ⇑ ∶ ty (A ⇛ B)\<\\
\>                                  stepB = ΛR stepA in\<\\
\>                              let stepC : addpath Δ A ⊢ var x₁ ∶ ty A\<\\
\>                                  stepC = varR x₁ validΔAAE in\<\\
\>                              let stepD : addpath Δ A ⊢ appT ((ΛT A M) ⟦ σ' ⟧ ⇑ ⇑ ⇑) (var x₁) ∶ ty B\<\\
\>                                  stepD = appR stepB stepC in\<\\
\>                              stepD)\<\\
\>                        (sym-conv (osr-conv (subst (λ a → appT ((ΛT A M ⟦ σ ⟧) ⇑ ⇑ ⇑) (var x₂) ⇒ a) (let open ≡-Reasoning in\<\\
\>                           M ⟦ Sub↑ \_ σ ⟧ 〈 Rep↑ \_ upRep 〉 〈 Rep↑ \_ upRep 〉 〈 Rep↑ \_ upRep 〉 ⟦ x₀:= (var x₂) ⟧\<\\
\>                         ≡⟨⟨ sub-compSR (M ⟦ Sub↑ \_ σ ⟧ 〈 Rep↑ \_ upRep 〉 〈 Rep↑ \_ upRep 〉) ⟩⟩\<\\
\>                           M ⟦ Sub↑ \_ σ ⟧ 〈 Rep↑ \_ upRep 〉 〈 Rep↑ \_ upRep 〉 ⟦ x₀:= (var x₂) •SR Rep↑ \_ upRep ⟧\<\\
\>                         ≡⟨⟨ sub-compSR (M ⟦ Sub↑ \_ σ ⟧ 〈 Rep↑ \_ upRep 〉) ⟩⟩\<\\
\>                           M ⟦ Sub↑ \_ σ ⟧ 〈 Rep↑ \_ upRep 〉 ⟦ x₀:= (var x₂) •SR Rep↑ \_ upRep •SR Rep↑ \_ upRep ⟧\<\\
\>                         ≡⟨⟨ sub-compSR (M ⟦ Sub↑ \_ σ ⟧) ⟩⟩\<\\
\>                           M ⟦ Sub↑ \_ σ ⟧ ⟦ x₀:= (var x₂) •SR Rep↑ \_ upRep •SR Rep↑ \_ upRep •SR Rep↑ \_ upRep ⟧\<\\
\>                         ≡⟨⟨ sub-comp M ⟩⟩\<\\
\>                           M ⟦ x₀:= (var x₂) •SR Rep↑ \_ upRep •SR Rep↑ \_ upRep •SR Rep↑ \_ upRep • Sub↑ \_ σ ⟧\<\\
\>                         ≡⟨ sub-congr M aux₃ ⟩\<\\
\>                           M ⟦ sub↖ σ ⟧\<\\
\>                           ∎) (redex ?)))) \<\\
\>                         (sym-conv (osr-conv (subst (λ a → appT ((ΛT A M ⟦ σ' ⟧) ⇑ ⇑ ⇑) (var x₁) ⇒ a) \<\\
\>                         (let open ≡-Reasoning in\<\\
\>                           M ⟦ Sub↑ \_ σ' ⟧ 〈 Rep↑ \_ upRep 〉 〈 Rep↑ \_ upRep 〉 〈 Rep↑ \_ upRep 〉 ⟦ x₀:= (var x₁) ⟧\<\\
\>                         ≡⟨⟨ sub-compSR (M ⟦ Sub↑ \_ σ' ⟧ 〈 Rep↑ \_ upRep 〉 〈 Rep↑ \_ upRep 〉) ⟩⟩\<\\
\>                           M ⟦ Sub↑ \_ σ' ⟧ 〈 Rep↑ \_ upRep 〉 〈 Rep↑ \_ upRep 〉 ⟦ x₀:= (var x₁) •SR Rep↑ \_ upRep ⟧\<\\
\>                         ≡⟨⟨ sub-compSR (M ⟦ Sub↑ \_ σ' ⟧ 〈 Rep↑ \_ upRep 〉) ⟩⟩\<\\
\>                           M ⟦ Sub↑ \_ σ' ⟧ 〈 Rep↑ \_ upRep 〉 ⟦ x₀:= (var x₁) •SR Rep↑ \_ upRep •SR Rep↑ \_ upRep ⟧\<\\
\>                         ≡⟨⟨ sub-compSR (M ⟦ Sub↑ \_ σ' ⟧) ⟩⟩\<\\
\>                           M ⟦ Sub↑ \_ σ' ⟧ ⟦ x₀:= (var x₁) •SR Rep↑ \_ upRep •SR Rep↑ \_ upRep •SR Rep↑ \_ upRep ⟧\<\\
\>                         ≡⟨⟨ sub-comp M ⟩⟩\<\\
\>                           M ⟦ x₀:= (var x₁) •SR Rep↑ \_ upRep •SR Rep↑ \_ upRep •SR Rep↑ \_ upRep • Sub↑ \_ σ' ⟧\<\\
\>                         ≡⟨ sub-congr M aux₄ ⟩\<\\
\>                           M ⟦ sub↗ σ' ⟧\<\\
\>                           ∎) \<\\
\>                         (redex ?))))))\<\\
\>    (λ W Θ N N' Q ρ ρ∶Δ⇒Θ N∈EΘA N'∈EΘA Q∈EΘN≡N' → \<\\
\>    let validΘ : valid Θ\<\\
\>        validΘ = Context-Validity (E-typed N∈EΘA) in\<\\
\>    let σ₁ : Sub (U , -Term) W\<\\
\>        σ₁ = x₀:= N •SR Rep↑ -Term ρ • Sub↑ -Term σ in\<\\
\>    let σ₁∶Γ,A⇒Θ : σ₁ ∶ Γ ,T A ⇒C Θ\<\\
\>        σ₁∶Γ,A⇒Θ = compC (compSRC (botsubC N∈EΘA) (Rep↑-typed ρ∶Δ⇒Θ)) (Sub↑C σ∶Γ⇒CΔ) in\<\\
\>    let σ₂ : Sub (U , -Term) W\<\\
\>        σ₂ = x₀:= N' •SR Rep↑ -Term ρ • Sub↑ -Term σ' in\<\\
\>    let σ₂∶Γ,A⇒Θ : σ₂ ∶ Γ ,T A ⇒C Θ\<\\
\>        σ₂∶Γ,A⇒Θ = compC (compSRC (botsubC N'∈EΘA) (Rep↑-typed ρ∶Δ⇒Θ)) (Sub↑C σ'∶Γ⇒CΔ) in --REFACTOR Common pattern\<\\
\>    let ρ' = Rep↑ -Path (Rep↑ -Term (Rep↑ -Term ρ)) in\<\\
\>    let step1 : x₀:= N • Sub↑ -Term (ρ •RS σ) ∼ σ₁\<\\
\>        step1 = sub-trans (comp-congr Sub↑-compRS) \<\\
\>                  (assocRSSR \{ρ = x₀:= N\} \{σ = Rep↑ -Term ρ\} \{τ = Sub↑ -Term σ\}) in\<\\
\>    let step2 : x₀:= N' • Sub↑ -Term (ρ •RS σ') ∼ σ₂\<\\
\>        step2 = sub-trans (comp-congr Sub↑-compRS) \<\\
\>                  (assocRSSR \{ρ = x₀:= N'\} \{σ = Rep↑ -Term ρ\} \{τ = Sub↑ -Term σ'\}) in\<\\
\>    let sub-rep-comp : ∀ (σ : Sub U V) (N : Term W) → M ⟦ x₀:= N •SR Rep↑ \_ ρ • Sub↑ \_ σ ⟧ ≡ M ⟦ Sub↑ \_ σ ⟧ 〈 Rep↑ \_ ρ 〉 ⟦ x₀:= N ⟧\<\\
\>        sub-rep-comp σ N = let open ≡-Reasoning in\<\\
\>             begin\<\\
\>               M ⟦ x₀:= N •SR Rep↑ -Term ρ • Sub↑ -Term σ ⟧\<\\
\>             ≡⟨ sub-comp M ⟩\<\\
\>               M ⟦ Sub↑ -Term σ ⟧ ⟦ x₀:= N •SR Rep↑ -Term ρ ⟧\<\\
\>             ≡⟨ sub-compSR (M ⟦ Sub↑ -Term σ ⟧) ⟩\<\\
\>               M ⟦ Sub↑ -Term σ ⟧ 〈 Rep↑ -Term ρ 〉 ⟦ x₀:= N ⟧\<\\
\>             ∎ in\<\\
\>    let ih : EE Θ (M ⟦ σ₁ ⟧ ≡〈 B 〉 M ⟦ σ₂ ⟧) \<\\
\>                  (M ⟦⟦ extendPS (ρ •RP τ) Q ∶ σ₁ ∼ σ₂ ⟧⟧)\<\\
\>        ih = (Computable-Path-Substitution (U , -Term) W (extendPS (ρ •RP τ) Q) σ₁ σ₂ (Γ ,T A) Θ \_ \_ σ₁∶Γ,A⇒Θ σ₂∶Γ,A⇒Θ\<\\
\>             (change-ends \{σ = x₀:= N' • Sub↑ -Term (ρ •RS σ')\} \{σ' = σ₂\} (extendPS-typedC (compRP-typedC \{ρ = ρ\} \{τ\} \{σ\} \{σ'\} τ∶σ∼σ' ρ∶Δ⇒Θ) \<\\
\>               Q∈EΘN≡N')\<\\
\>                 step1 step2) Γ,A⊢M∶B validΘ) in\<\\
\>    let Δ,A⊢Mσ∶B : Δ ,T A ⊢ M ⟦ Sub↑ \_ σ ⟧ ∶ ty B\<\\
\>        Δ,A⊢Mσ∶B = Substitution Γ,A⊢M∶B (ctxTR validΔ) (Sub↑-typed σ∶Γ⇒Δ) in\<\\
\>    let Δ,A⊢Mσ'∶B : Δ ,T A ⊢ M ⟦ Sub↑ \_ σ' ⟧ ∶ ty B\<\\
\>        Δ,A⊢Mσ'∶B = Substitution Γ,A⊢M∶B (ctxTR validΔ) (Sub↑-typed σ'∶Γ⇒Δ) in\<\\
\>    let Θ,A⊢Mσ∶B : Θ ,T A ⊢ M ⟦ Sub↑ \_ σ ⟧ 〈 Rep↑ \_ ρ 〉 ∶ ty B\<\\
\>        Θ,A⊢Mσ∶B = Weakening Δ,A⊢Mσ∶B (ctxTR validΘ) (Rep↑-typed ρ∶Δ⇒Θ) in\<\\
\>    let Θ,A⊢Mσ'∶B : Θ ,T A ⊢ M ⟦ Sub↑ \_ σ' ⟧ 〈 Rep↑ \_ ρ 〉 ∶ ty B\<\\
\>        Θ,A⊢Mσ'∶B = Weakening Δ,A⊢Mσ'∶B (ctxTR validΘ) (Rep↑-typed ρ∶Δ⇒Θ) in --TODO Common pattern\<\\
\>    let Θ⊢N∶A : Θ ⊢ N ∶ ty A\<\\
\>        Θ⊢N∶A = E-typed N∈EΘA in\<\\
\>    let Θ⊢N'∶A : Θ ⊢ N' ∶ ty A\<\\
\>        Θ⊢N'∶A = E-typed N'∈EΘA in\<\\
\>        expand-EE (conv-EE \<\\
\>          (subst (EE Θ (M ⟦ σ₁ ⟧ ≡〈 B 〉 M ⟦ σSR ⟧)) (let open ≡-Reasoning in\<\\
\>          begin\<\\
\>            M ⟦⟦ extendPS (ρ •RP τ) Q ∶ σ₁ ∼\<\\
\>                 σSR ⟧⟧\<\\
\>          ≡⟨⟨ pathsub-cong M ∼∼-refl step1 step2 ⟩⟩\<\\
\>            M ⟦⟦ extendPS (ρ •RP τ) Q ∶ x₀:= N • Sub↑ -Term (ρ •RS σ) ∼\<\\
\>                 x₀:= N' • Sub↑ -Term (ρ •RS σ') ⟧⟧\<\\
\>          ≡⟨ pathsub-extendPS M ⟩\<\\
\>            M ⟦⟦ pathsub↑ (ρ •RP τ) ∶ sub↖ (ρ •RS σ) ∼ sub↗ (ρ •RS σ') ⟧⟧ ⟦ x₀:= N • x₀:= (N' ⇑) • x₀:= (Q ⇑ ⇑) ⟧\<\\
\>          ≡⟨ sub-congl (pathsub-cong M pathsub↑-compRP sub↖-comp₁ sub↗-comp₁) ⟩\<\\
\>            M ⟦⟦ ρ' •RP pathsub↑ τ ∶ ρ' •RS sub↖ σ ∼ ρ' •RS sub↗ σ' ⟧⟧ ⟦ x₀:= N • x₀:= (N' ⇑) • x₀:= (Q ⇑ ⇑) ⟧\<\\
\>          ≡⟨ sub-congl (pathsub-compRP M) ⟩\<\\
\>            (M ⟦⟦ pathsub↑ τ ∶ sub↖ σ ∼ sub↗ σ' ⟧⟧) 〈 ρ' 〉 ⟦ x₀:= N • x₀:= (N' ⇑) • x₀:= (Q ⇑ ⇑) ⟧\<\\
\>          ∎) ih) \<\\
\>          (sym-conv (osr-conv (subst (λ a → appT ((ΛT A M) ⟦ σ ⟧ 〈 ρ 〉) N ⇒ a) (sym (sub-rep-comp σ N)) (redex ?)))) \<\\
\>          (sym-conv (osr-conv (subst (λ a → appT ((ΛT A M) ⟦ σ' ⟧ 〈 ρ 〉) N' ⇒ a) (sym (sub-rep-comp σ' N')) (redex ?)))) --REFACTOR Duplication\<\\
\>          (appR (ΛR Θ,A⊢Mσ∶B) Θ⊢N∶A) \<\\
\>          (appR (ΛR Θ,A⊢Mσ'∶B) (E-typed N'∈EΘA)))\<\\
\>        (let step3 : addpath Δ A ⊢\<\\
\>                         M ⟦⟦ pathsub↑ τ ∶ sub↖ σ ∼ sub↗ σ' ⟧⟧\<\\
\>                         ∶ M ⟦ sub↖ σ ⟧ ≡〈 B 〉 M ⟦ sub↗ σ' ⟧\<\\
\>             step3 = Path-Substitution Γ,A⊢M∶B (pathsub↑-typed (pathsubC-typed \{τ = τ\} \{σ\} \{σ'\} \{Γ\} \{Δ\} τ∶σ∼σ')) \<\\
\>                     sub↖σ-typed sub↗σ'-typed validΔAAE in\<\\
\>        let step4 : addpath Θ A ⊢\<\\
\>                    M ⟦⟦ pathsub↑ τ ∶ sub↖ σ ∼ sub↗ σ' ⟧⟧ 〈 ρ' 〉\<\\
\>                  ∶ M ⟦ sub↖ σ ⟧ 〈 ρ' 〉 ≡〈 B 〉 M ⟦ sub↗ σ' ⟧ 〈 ρ' 〉\<\\
\>            step4 = Weakening step3 \<\\
\>                    (ctxER (varR x₁ (ctxTR (ctxTR validΘ)))\<\\
\>                    (varR x₀ (ctxTR (ctxTR validΘ))))\<\\
\>                    (Rep↑-typed (Rep↑-typed (Rep↑-typed ρ∶Δ⇒Θ))) in\<\\
\>        let step5 : ∀ σ x → σ ∶ Γ ⇒ Δ → typeof x (addpath Θ A) ≡ ty A → addpath Θ A ⊢\<\\
\>                    appT ((ΛT A M) ⟦ σ ⟧ 〈 ρ 〉 ⇑ ⇑ ⇑) (var x) ∶ ty B\<\\
\>            step5 σ x σ∶Γ⇒Θ x∶A∈ΘA = appR \<\\
\>                           (ΛR (subst (λ a → addpath Θ A ,T A ⊢ a ∶ ty B) \<\\
\>                           (trans (sub-compRS M) (trans (rep-comp (M ⟦ Sub↑ \_ σ ⟧))\<\\
\>                           (trans (rep-comp (M ⟦ Sub↑ \_ σ ⟧ 〈 Rep↑ \_ ρ 〉)) \<\\
\>                             (rep-comp (M ⟦ Sub↑ \_ σ ⟧ 〈 Rep↑ \_ ρ 〉 〈 Rep↑ \_ upRep 〉)))))\<\\
\>                         (Substitution \{σ = Rep↑ \_ upRep •R Rep↑ \_ upRep •R Rep↑ \_ upRep •R Rep↑ \_ ρ •RS Sub↑ \_ σ\} Γ,A⊢M∶B \<\\
\>                         (ctxTR (ctxER (varR x₁ (ctxTR (ctxTR validΘ))) (varR x₀ (ctxTR (ctxTR validΘ)))))\<\\
\>                         (compRS-typed\<\\
\>                            \{ρ = Rep↑ \_ upRep •R Rep↑ \_ upRep •R Rep↑ \_ upRep •R Rep↑ \_ ρ\}\<\\
\>                            \{σ = Sub↑ \_ σ\} \<\\
\>                            (compR-typed \{ρ = Rep↑ \_ upRep •R Rep↑ \_ upRep •R Rep↑ \_ upRep\}\<\\
\>                              \{σ = Rep↑ \_ ρ\}\<\\
\>                              (compR-typed \{ρ = Rep↑ \_ upRep •R Rep↑ \_ upRep\} \{σ = Rep↑ \_ upRep\}\<\\
\>                                (compR-typed \{ρ = Rep↑ \_ upRep\} \{σ = Rep↑ \_ upRep\} (Rep↑-typed upRep-typed) (Rep↑-typed upRep-typed)) (Rep↑-typed upRep-typed)) \<\\
\>                            (Rep↑-typed ρ∶Δ⇒Θ))\<\\
\>                         (Sub↑-typed σ∶Γ⇒Θ)))))\<\\
\>                         (change-type (varR x (ctxER (varR x₁ (ctxTR (ctxTR validΘ))) (varR x₀ (ctxTR (ctxTR validΘ))))) x∶A∈ΘA) in --TODO Extract last line as lemma\<\\
\>             let step6 : addpath Θ A ⊢\<\\
\>                         M ⟦⟦ pathsub↑ τ ∶ sub↖ σ ∼ sub↗ σ' ⟧⟧ 〈 ρ' 〉\<\\
\>                         ∶ appT ((ΛT A M) ⟦ σ ⟧ 〈 ρ 〉 ⇑ ⇑ ⇑) (var x₂) ≡〈 B 〉 appT ((ΛT A M) ⟦ σ' ⟧ 〈 ρ 〉 ⇑ ⇑ ⇑) (var x₁)\<\\
\>                 step6 = convER step4 (step5 σ x₂ σ∶Γ⇒Δ refl) (step5 σ' x₁ σ'∶Γ⇒Δ refl)\<\\
\>                         (subst (λ a → a ≃ appT (((ΛT A M ⟦ σ ⟧) 〈 ρ 〉) ⇑ ⇑ ⇑) (var x₂)) \<\\
\>                         (let open ≡-Reasoning in\<\\
\>                           M ⟦ Sub↑ \_ σ ⟧ 〈 Rep↑ \_ ρ 〉 〈 Rep↑ \_ upRep 〉 〈 Rep↑ \_ upRep 〉 〈 Rep↑ \_ upRep 〉 ⟦ x₀:= (var x₂) ⟧\<\\
\>                         ≡⟨⟨ sub-compSR (M ⟦ Sub↑ \_ σ ⟧ 〈 Rep↑ \_ ρ 〉 〈 Rep↑ \_ upRep 〉 〈 Rep↑ \_ upRep 〉) ⟩⟩\<\\
\>                           M ⟦ Sub↑ \_ σ ⟧ 〈 Rep↑ \_ ρ 〉 〈 Rep↑ \_ upRep 〉 〈 Rep↑ \_ upRep 〉 ⟦ x₀:= (var x₂) •SR Rep↑ \_ upRep ⟧\<\\
\>                         ≡⟨⟨ sub-compSR (M ⟦ Sub↑ \_ σ ⟧ 〈 Rep↑ \_ ρ 〉 〈 Rep↑ \_ upRep 〉) ⟩⟩\<\\
\>                           M ⟦ Sub↑ \_ σ ⟧ 〈 Rep↑ \_ ρ 〉 〈 Rep↑ \_ upRep 〉 ⟦ x₀:= (var x₂) •SR Rep↑ \_ upRep •SR Rep↑ \_ upRep ⟧\<\\
\>                         ≡⟨⟨ sub-compSR (M ⟦ Sub↑ \_ σ ⟧ 〈 Rep↑ \_ ρ 〉) ⟩⟩\<\\
\>                           M ⟦ Sub↑ \_ σ ⟧ 〈 Rep↑ \_ ρ 〉 ⟦ x₀:= (var x₂) •SR Rep↑ \_ upRep •SR Rep↑ \_ upRep •SR Rep↑ \_ upRep ⟧\<\\
\>                         ≡⟨⟨ sub-compSR (M ⟦ Sub↑ \_ σ ⟧) ⟩⟩\<\\
\>                           M ⟦ Sub↑ \_ σ ⟧ ⟦ x₀:= (var x₂) •SR Rep↑ \_ upRep •SR Rep↑ \_ upRep •SR Rep↑ \_ upRep •SR Rep↑ \_ ρ ⟧\<\\
\>                         ≡⟨⟨ sub-comp M ⟩⟩\<\\
\>                           M ⟦ x₀:= (var x₂) •SR Rep↑ \_ upRep •SR Rep↑ \_ upRep •SR Rep↑ \_ upRep •SR Rep↑ \_ ρ • Sub↑ \_ σ ⟧\<\\
\>                         ≡⟨ sub-congr M aux ⟩\<\\
\>                           M ⟦ Rep↑ \_ (Rep↑ \_ (Rep↑ \_ ρ)) •RS sub↖ σ ⟧\<\\
\>                         ≡⟨ sub-compRS M ⟩ \<\\
\>                           M ⟦ sub↖ σ ⟧ 〈 Rep↑ \_ (Rep↑ \_ (Rep↑ \_ ρ)) 〉\<\\
\>                           ∎)\<\\
\>                           (sym-conv (osr-conv (redex ?)))) \<\\
\>                         (subst (λ a → a ≃ appT (((ΛT A M ⟦ σ' ⟧) 〈 ρ 〉) ⇑ ⇑ ⇑) (var x₁)) \<\\
\>                           (let open ≡-Reasoning in \<\\
\>                           M ⟦ Sub↑ \_ σ' ⟧ 〈 Rep↑ \_ ρ 〉 〈 Rep↑ \_ upRep 〉 〈 Rep↑ \_ upRep 〉 〈 Rep↑ \_ upRep 〉 ⟦ x₀:= (var x₁) ⟧\<\\
\>                         ≡⟨⟨ sub-compSR (M ⟦ Sub↑ \_ σ' ⟧ 〈 Rep↑ \_ ρ 〉 〈 Rep↑ \_ upRep 〉 〈 Rep↑ \_ upRep 〉) ⟩⟩\<\\
\>                           M ⟦ Sub↑ \_ σ' ⟧ 〈 Rep↑ \_ ρ 〉 〈 Rep↑ \_ upRep 〉 〈 Rep↑ \_ upRep 〉 ⟦ x₀:= (var x₁) •SR Rep↑ \_ upRep ⟧\<\\
\>                         ≡⟨⟨ sub-compSR (M ⟦ Sub↑ \_ σ' ⟧ 〈 Rep↑ \_ ρ 〉 〈 Rep↑ \_ upRep 〉) ⟩⟩\<\\
\>                           M ⟦ Sub↑ \_ σ' ⟧ 〈 Rep↑ \_ ρ 〉 〈 Rep↑ \_ upRep 〉 ⟦ x₀:= (var x₁) •SR Rep↑ \_ upRep •SR Rep↑ \_ upRep ⟧\<\\
\>                         ≡⟨⟨ sub-compSR (M ⟦ Sub↑ \_ σ' ⟧ 〈 Rep↑ \_ ρ 〉) ⟩⟩\<\\
\>                           M ⟦ Sub↑ \_ σ' ⟧ 〈 Rep↑ \_ ρ 〉 ⟦ x₀:= (var x₁) •SR Rep↑ \_ upRep •SR Rep↑ \_ upRep •SR Rep↑ \_ upRep ⟧\<\\
\>                         ≡⟨⟨ sub-compSR (M ⟦ Sub↑ \_ σ' ⟧) ⟩⟩\<\\
\>                           M ⟦ Sub↑ \_ σ' ⟧ ⟦ x₀:= (var x₁) •SR Rep↑ \_ upRep •SR Rep↑ \_ upRep •SR Rep↑ \_ upRep •SR Rep↑ \_ ρ ⟧\<\\
\>                         ≡⟨⟨ sub-comp M ⟩⟩\<\\
\>                           M ⟦ x₀:= (var x₁) •SR Rep↑ \_ upRep •SR Rep↑ \_ upRep •SR Rep↑ \_ upRep •SR Rep↑ \_ ρ • Sub↑ \_ σ' ⟧\<\\
\>                         ≡⟨ sub-congr M aux₂ ⟩\<\\
\>                           M ⟦ Rep↑ \_ (Rep↑ \_ (Rep↑ \_ ρ)) •RS sub↗ σ' ⟧\<\\
\>                         ≡⟨ sub-compRS M ⟩ \<\\
\>                           M ⟦ sub↗ σ' ⟧ 〈 Rep↑ \_ (Rep↑ \_ (Rep↑ \_ ρ)) 〉\<\\
\>                           ∎)\<\\
\>                           (sym-conv (osr-conv (redex ?)))) in\<\\
\>      app*R (E-typed N∈EΘA) (E-typed N'∈EΘA) \<\\
\>      (lllR step6) (EE-typed Q∈EΘN≡N'))\<\\
\>      ?) where\<\\
\>    aux : ∀ \{U\} \{V\} \{W\} \{ρ : Rep V W\} \{σ : Sub U V\} → \<\\
\>        x₀:= (var x₂) •SR Rep↑ \_ upRep •SR Rep↑ \_ upRep •SR Rep↑ \_ upRep •SR Rep↑ \_ ρ • Sub↑ \_ σ ∼ Rep↑ \_ (Rep↑ \_ (Rep↑ \_ ρ)) •RS sub↖ σ\<\\
\>    aux x₀ = refl\<\\
\>    aux \{ρ = ρ\} \{σ\} (↑ x) = let open ≡-Reasoning in \<\\
\>      begin\<\\
\>        σ \_ x ⇑ ⟦ x₀:= (var x₂) •SR Rep↑ -Term upRep •SR Rep↑ -Term upRep •SR\<\\
\>       Rep↑ -Term upRep\<\\
\>       •SR Rep↑ -Term ρ ⟧\<\\
\>      ≡⟨ sub-compSR (σ \_ x ⇑) ⟩\<\\
\>        σ \_ x ⇑ 〈 Rep↑ \_ ρ 〉 ⟦ x₀:= (var x₂) •SR Rep↑ -Term upRep •SR Rep↑ -Term upRep •SR Rep↑ -Term upRep ⟧\<\\
\>      ≡⟨ sub-congl (Rep↑-upRep (σ \_ x)) ⟩\<\\
\>        σ \_ x 〈 ρ 〉 ⇑ ⟦ x₀:= (var x₂) •SR Rep↑ -Term upRep •SR Rep↑ -Term upRep •SR Rep↑ -Term upRep ⟧\<\\
\>      ≡⟨ sub-compSR (σ \_ x 〈 ρ 〉 ⇑) ⟩\<\\
\>        σ \_ x 〈 ρ 〉 ⇑ 〈 Rep↑ \_ upRep 〉 ⟦ x₀:= (var x₂) •SR Rep↑ -Term upRep •SR Rep↑ -Term upRep ⟧\<\\
\>      ≡⟨ sub-congl (Rep↑-upRep (σ \_ x 〈 ρ 〉)) ⟩\<\\
\>        σ \_ x 〈 ρ 〉 ⇑ ⇑ ⟦ x₀:= (var x₂) •SR Rep↑ -Term upRep •SR Rep↑ -Term upRep ⟧\<\\
\>      ≡⟨ sub-compSR (σ \_ x 〈 ρ 〉 ⇑ ⇑) ⟩\<\\
\>        σ \_ x 〈 ρ 〉 ⇑ ⇑ 〈 Rep↑ \_ upRep 〉 ⟦ x₀:= (var x₂) •SR Rep↑ -Term upRep ⟧\<\\
\>      ≡⟨ sub-congl (Rep↑-upRep (σ \_ x 〈 ρ 〉 ⇑)) ⟩\<\\
\>        σ \_ x 〈 ρ 〉 ⇑ ⇑ ⇑ ⟦ x₀:= (var x₂) •SR Rep↑ -Term upRep ⟧\<\\
\>      ≡⟨ sub-compSR (σ \_ x 〈 ρ 〉 ⇑ ⇑ ⇑) ⟩\<\\
\>        σ \_ x 〈 ρ 〉 ⇑ ⇑ ⇑ 〈 Rep↑ -Term upRep 〉 ⟦ x₀:= (var x₂) ⟧\<\\
\>      ≡⟨ sub-congl (Rep↑-upRep (σ \_ x 〈 ρ 〉 ⇑ ⇑)) ⟩\<\\
\>        σ \_ x 〈 ρ 〉 ⇑ ⇑ ⇑ ⇑ ⟦ x₀:= (var x₂) ⟧\<\\
\>      ≡⟨ botsub-upRep (σ \_ x 〈 ρ 〉 ⇑ ⇑ ⇑) ⟩\<\\
\>        σ \_ x 〈 ρ 〉 ⇑ ⇑ ⇑\<\\
\>      ≡⟨⟨ Rep↑-upRep₃ (σ \_ x) ⟩⟩\<\\
\>        σ \_ x ⇑ ⇑ ⇑ 〈 Rep↑ \_ (Rep↑ \_ (Rep↑ \_ ρ)) 〉\<\\
\>      ∎\<\\
\>    aux₂ : ∀ \{U\} \{V\} \{W\} \{ρ : Rep V W\} \{σ : Sub U V\} → \<\\
\>        x₀:= (var x₁) •SR Rep↑ \_ upRep •SR Rep↑ \_ upRep •SR Rep↑ \_ upRep •SR Rep↑ \_ ρ • Sub↑ \_ σ ∼ Rep↑ \_ (Rep↑ \_ (Rep↑ \_ ρ)) •RS sub↗ σ\<\\
\>    aux₂ x₀ = refl\<\\
\>    aux₂ \{ρ = ρ\} \{σ\} (↑ x) = let open ≡-Reasoning in \<\\
\>      begin\<\\
\>        σ \_ x ⇑ ⟦ x₀:= (var x₁) •SR Rep↑ -Term upRep •SR Rep↑ -Term upRep •SR\<\\
\>       Rep↑ -Term upRep\<\\
\>       •SR Rep↑ -Term ρ ⟧\<\\
\>      ≡⟨ sub-compSR (σ \_ x ⇑) ⟩\<\\
\>        σ \_ x ⇑ 〈 Rep↑ \_ ρ 〉 ⟦ x₀:= (var x₁) •SR Rep↑ -Term upRep •SR Rep↑ -Term upRep •SR Rep↑ -Term upRep ⟧\<\\
\>      ≡⟨ sub-congl (Rep↑-upRep (σ \_ x)) ⟩\<\\
\>        σ \_ x 〈 ρ 〉 ⇑ ⟦ x₀:= (var x₁) •SR Rep↑ -Term upRep •SR Rep↑ -Term upRep •SR Rep↑ -Term upRep ⟧\<\\
\>      ≡⟨ sub-compSR (σ \_ x 〈 ρ 〉 ⇑) ⟩\<\\
\>        σ \_ x 〈 ρ 〉 ⇑ 〈 Rep↑ \_ upRep 〉 ⟦ x₀:= (var x₁) •SR Rep↑ -Term upRep •SR Rep↑ -Term upRep ⟧\<\\
\>      ≡⟨ sub-congl (Rep↑-upRep (σ \_ x 〈 ρ 〉)) ⟩\<\\
\>        σ \_ x 〈 ρ 〉 ⇑ ⇑ ⟦ x₀:= (var x₁) •SR Rep↑ -Term upRep •SR Rep↑ -Term upRep ⟧\<\\
\>      ≡⟨ sub-compSR (σ \_ x 〈 ρ 〉 ⇑ ⇑) ⟩\<\\
\>        σ \_ x 〈 ρ 〉 ⇑ ⇑ 〈 Rep↑ \_ upRep 〉 ⟦ x₀:= (var x₁) •SR Rep↑ -Term upRep ⟧\<\\
\>      ≡⟨ sub-congl (Rep↑-upRep (σ \_ x 〈 ρ 〉 ⇑)) ⟩\<\\
\>        σ \_ x 〈 ρ 〉 ⇑ ⇑ ⇑ ⟦ x₀:= (var x₁) •SR Rep↑ -Term upRep ⟧\<\\
\>      ≡⟨ sub-compSR (σ \_ x 〈 ρ 〉 ⇑ ⇑ ⇑) ⟩\<\\
\>        σ \_ x 〈 ρ 〉 ⇑ ⇑ ⇑ 〈 Rep↑ -Term upRep 〉 ⟦ x₀:= (var x₁) ⟧\<\\
\>      ≡⟨ sub-congl (Rep↑-upRep (σ \_ x 〈 ρ 〉 ⇑ ⇑)) ⟩\<\\
\>        σ \_ x 〈 ρ 〉 ⇑ ⇑ ⇑ ⇑ ⟦ x₀:= (var x₁) ⟧\<\\
\>      ≡⟨ botsub-upRep (σ \_ x 〈 ρ 〉 ⇑ ⇑ ⇑) ⟩\<\\
\>        σ \_ x 〈 ρ 〉 ⇑ ⇑ ⇑\<\\
\>      ≡⟨⟨ Rep↑-upRep₃ (σ \_ x) ⟩⟩\<\\
\>        σ \_ x ⇑ ⇑ ⇑ 〈 Rep↑ \_ (Rep↑ \_ (Rep↑ \_ ρ)) 〉\<\\
\>      ∎\<\\
\>    aux₃ : ∀ \{U\} \{V\} \{σ : Sub U V\} → \<\\
\>        x₀:= (var x₂) •SR Rep↑ \_ upRep •SR Rep↑ \_ upRep •SR Rep↑ \_ upRep • Sub↑ \_ σ ∼ sub↖ σ\<\\
\>    aux₃ x₀ = refl\<\\
\>    aux₃ \{σ = σ\} (↑ x) = let open ≡-Reasoning in \<\\
\>      begin\<\\
\>        σ \_ x ⇑ ⟦ x₀:= (var x₂) •SR Rep↑ -Term upRep •SR Rep↑ -Term upRep •SR Rep↑ -Term upRep ⟧\<\\
\>      ≡⟨ sub-compSR (σ \_ x ⇑) ⟩\<\\
\>        σ \_ x ⇑ 〈 Rep↑ \_ upRep 〉 ⟦ x₀:= (var x₂) •SR Rep↑ -Term upRep •SR Rep↑ -Term upRep ⟧\<\\
\>      ≡⟨ sub-congl (Rep↑-upRep (σ \_ x)) ⟩\<\\
\>        σ \_ x ⇑ ⇑ ⟦ x₀:= (var x₂) •SR Rep↑ -Term upRep •SR Rep↑ -Term upRep ⟧\<\\
\>      ≡⟨ sub-compSR (σ \_ x  ⇑ ⇑) ⟩\<\\
\>        σ \_ x  ⇑ ⇑ 〈 Rep↑ \_ upRep 〉 ⟦ x₀:= (var x₂) •SR Rep↑ -Term upRep ⟧\<\\
\>      ≡⟨ sub-congl (Rep↑-upRep (σ \_ x  ⇑)) ⟩\<\\
\>        σ \_ x  ⇑ ⇑ ⇑ ⟦ x₀:= (var x₂) •SR Rep↑ -Term upRep ⟧\<\\
\>      ≡⟨ sub-compSR (σ \_ x  ⇑ ⇑ ⇑) ⟩\<\\
\>        σ \_ x  ⇑ ⇑ ⇑ 〈 Rep↑ -Term upRep 〉 ⟦ x₀:= (var x₂) ⟧\<\\
\>      ≡⟨ sub-congl (Rep↑-upRep (σ \_ x  ⇑ ⇑)) ⟩\<\\
\>        σ \_ x  ⇑ ⇑ ⇑ ⇑ ⟦ x₀:= (var x₂) ⟧\<\\
\>      ≡⟨ botsub-upRep (σ \_ x  ⇑ ⇑ ⇑) ⟩\<\\
\>        σ \_ x  ⇑ ⇑ ⇑\<\\
\>      ∎\<\\
\>    aux₄ : ∀ \{U\} \{V\} \{σ : Sub U V\} → \<\\
\>        x₀:= (var x₁) •SR Rep↑ \_ upRep •SR Rep↑ \_ upRep •SR Rep↑ \_ upRep • Sub↑ \_ σ ∼ sub↗ σ\<\\
\>    aux₄ x₀ = refl\<\\
\>    aux₄ \{σ = σ\} (↑ x) = let open ≡-Reasoning in \<\\
\>      begin\<\\
\>        σ \_ x ⇑ ⟦ x₀:= (var x₁) •SR Rep↑ -Term upRep •SR Rep↑ -Term upRep •SR Rep↑ -Term upRep ⟧\<\\
\>      ≡⟨ sub-compSR (σ \_ x  ⇑) ⟩\<\\
\>        σ \_ x  ⇑ 〈 Rep↑ \_ upRep 〉 ⟦ x₀:= (var x₁) •SR Rep↑ -Term upRep •SR Rep↑ -Term upRep ⟧\<\\
\>      ≡⟨ sub-congl (Rep↑-upRep (σ \_ x )) ⟩\<\\
\>        σ \_ x  ⇑ ⇑ ⟦ x₀:= (var x₁) •SR Rep↑ -Term upRep •SR Rep↑ -Term upRep ⟧\<\\
\>      ≡⟨ sub-compSR (σ \_ x  ⇑ ⇑) ⟩\<\\
\>        σ \_ x  ⇑ ⇑ 〈 Rep↑ \_ upRep 〉 ⟦ x₀:= (var x₁) •SR Rep↑ -Term upRep ⟧\<\\
\>      ≡⟨ sub-congl (Rep↑-upRep (σ \_ x  ⇑)) ⟩\<\\
\>        σ \_ x  ⇑ ⇑ ⇑ ⟦ x₀:= (var x₁) •SR Rep↑ -Term upRep ⟧\<\\
\>      ≡⟨ sub-compSR (σ \_ x  ⇑ ⇑ ⇑) ⟩\<\\
\>        σ \_ x  ⇑ ⇑ ⇑ 〈 Rep↑ -Term upRep 〉 ⟦ x₀:= (var x₁) ⟧\<\\
\>      ≡⟨ sub-congl (Rep↑-upRep (σ \_ x  ⇑ ⇑)) ⟩\<\\
\>        σ \_ x  ⇑ ⇑ ⇑ ⇑ ⟦ x₀:= (var x₁) ⟧\<\\
\>      ≡⟨ botsub-upRep (σ \_ x  ⇑ ⇑ ⇑) ⟩\<\\
\>        σ \_ x  ⇑ ⇑ ⇑\<\\
\>      ∎ -\}}\<%
\end{code}
}

\begin{corollary}[Strong Normalization]
Every well-typed term, proof and path is strongly normalizing.
\end{corollary}

\begin{proof}
We apply the theorem with $\sigma$ the identity substitution.  The identity substitution is computable
by Lemma \ref{lm:var-compute}.
\end{proof}

\begin{code}%
\>\AgdaKeyword{postulate} \AgdaPostulate{Strong-Normalization} \AgdaSymbol{:} \AgdaSymbol{∀} \AgdaBound{V} \AgdaBound{K} \AgdaSymbol{(}\AgdaBound{Γ} \AgdaSymbol{:} \AgdaDatatype{Context} \AgdaBound{V}\AgdaSymbol{)} \<[55]%
\>[55]\<%
\\
\>[0]\AgdaIndent{31}{}\<[31]%
\>[31]\AgdaSymbol{(}\AgdaBound{M} \AgdaSymbol{:} \AgdaFunction{Expression} \AgdaBound{V} \AgdaSymbol{(}\AgdaInductiveConstructor{varKind} \AgdaBound{K}\AgdaSymbol{))} \AgdaBound{A} \AgdaSymbol{→} \AgdaBound{Γ} \AgdaDatatype{⊢} \AgdaBound{M} \AgdaDatatype{∶} \AgdaBound{A} \AgdaSymbol{→} \AgdaDatatype{SN} \AgdaBound{M}\<%
\end{code}

\AgdaHide{
\begin{code}%
\>\AgdaComment{\{-Strong-Normalization V -Proof Γ δ φ Γ⊢δ∶φ = EP-SN \<\\
\>  (subst (EP Γ \_) sub-idOp\<\\
\>  (Computable-Proof-Substitution V V (idSub V) Γ Γ δ φ idSubC Γ⊢δ∶φ (Context-Validity Γ⊢δ∶φ)))\<\\
\>Strong-Normalization V -Term Γ M (app (-ty A) out) Γ⊢M∶A = E-SN A\<\\
\>  (subst (E Γ A) sub-idOp \<\\
\>  (Computable-Substitution V V (idSub V) Γ Γ M A idSubC Γ⊢M∶A (Context-Validity Γ⊢M∶A)))\<\\
\>Strong-Normalization V -Path Γ P E Γ⊢P∶E = EE-SN E \<\\
\>  (substSR (EE Γ) sub-idOp sub-idOp\<\\
\>  (Computable-Path-SubstitutionRS V V (idSub V) Γ Γ P E idSubC Γ⊢P∶E (Context-Validity Γ⊢P∶E)))-\}}\<%
\end{code}
}

\begin{corollary}[Consistency]
There is no proof $\delta$ such that $\vdash \delta : \bot$.
\end{corollary}

\AgdaHide{
\begin{code}%
\>\AgdaKeyword{postulate} \AgdaPostulate{Consistency'} \AgdaSymbol{:} \AgdaSymbol{∀} \AgdaSymbol{\{}\AgdaBound{M} \AgdaSymbol{:} \AgdaFunction{Proof} \AgdaInductiveConstructor{∅}\AgdaSymbol{\}} \AgdaSymbol{→} \AgdaDatatype{SN} \AgdaBound{M} \AgdaSymbol{→} \AgdaInductiveConstructor{〈〉} \AgdaDatatype{⊢} \AgdaBound{M} \AgdaDatatype{∶} \AgdaFunction{⊥} \AgdaSymbol{→} \AgdaDatatype{Empty}\<%
\\
\>\AgdaComment{-- Consistency' (SNI M SNM) ⊢M∶⊥ = \{!!\}}\<%
\end{code}
}

\begin{code}%
\>\AgdaKeyword{postulate} \AgdaPostulate{Consistency} \AgdaSymbol{:} \AgdaSymbol{∀} \AgdaSymbol{\{}\AgdaBound{M} \AgdaSymbol{:} \AgdaFunction{Proof} \AgdaInductiveConstructor{∅}\AgdaSymbol{\}} \AgdaSymbol{→} \AgdaInductiveConstructor{〈〉} \AgdaDatatype{⊢} \AgdaBound{M} \AgdaDatatype{∶} \AgdaFunction{⊥} \AgdaSymbol{→} \AgdaDatatype{Empty}\<%
\end{code}

\AgdaHide{
\begin{code}%
\>\AgdaComment{-- Consistency = \{!!\}}\<%
\end{code}
}
